Support for Isar structural proofs
Improved top-level parallelism.
Other numerous improvements.

Eval/eval_abduction_dir.py
@@ -3,6 +3,7 @@
 import argparse
 import csv
 import os
+import re
 import signal
 import shutil
 import subprocess
