Eval/generated/tbc/TIP15/TIP_list_weird_is_normal.thy
@@ -1,7 +1,0 @@
-(* This Isabelle theory is produced using the TIP tool offered at the following website: 
-     https://github.com/tip-org/tools 
-   This file was originally provided as part of TIP benchmark at the following website:
-     https://github.com/tip-org/benchmarks 
-   Yutaka Nagashima at CIIRC, CTU changed the TIP output theory file slightly 
-   to make it compatible with Isabelle2017.*)
-  
