SeLFiE/Example/More_SeLFiE_Assertion.thy
@@ -1,3 +1,9 @@
+(*  Title:      SeLFiE/Example/More_SeLFiE_Assertion.thy
+    Author:     Yutaka Nagashima
+
+Example SeLFiE assertions built from SeLFiE_Util, Eval_Syntactic_Sugar,
+Quantifier_Domain, and Pattern.
+*)
 theory More_SeLFiE_Assertion
 imports "../SeLFiE"
 begin
