SeLFiE/Example/Test_Some_AFPs.thy
@@ -1,3 +1,9 @@
+(*  Title:      SeLFiE/Example/Test_Some_AFPs.thy
+    Author:     Yutaka Nagashima
+
+Smoke-test theory that merely imports a handful of AFP entries, to check that
+they still load under the current Isabelle/AFP versions.
+*)
 theory Test_Some_AFPs
   imports
     "afp-2020-05-16/thys/KD_Tree/Nearest_Neighbors"
